[skip ci] pending LemmaScript change on JS trim

apps/web/src/utils/redirect.dfy
@@ -2,22 +2,32 @@
 
 datatype Option<T> = None | Some(value: T)
 
+predicate IsJSWhitespace(c: char)
+{
+  c == '\U{0009}' || c == '\U{000A}' || c == '\U{000B}' || c == '\U{000C}' || c == '\U{000D}' ||
+  c == '\U{0020}' || c == '\U{00A0}' || c == '\U{1680}' ||
+  ('\U{2000}' <= c <= '\U{200A}') ||
+  c == '\U{2028}' || c == '\U{2029}' || c == '\U{202F}' || c == '\U{205F}' ||
+  c == '\U{3000}' || c == '\U{FEFF}'
+}
+
 function StringTrimLeft(s: string): string
   ensures |StringTrimLeft(s)| <= |s|
-  ensures StringTrimLeft(s) == "" || (|StringTrimLeft(s)| > 0 && StringTrimLeft(s)[0] != ' ')
+  ensures StringTrimLeft(s) == "" || (|StringTrimLeft(s)| > 0 && !IsJSWhitespace(StringTrimLeft(s)[0]))
   decreases |s|
 {
   if |s| == 0 then ""
-  else if s[0] == ' ' then StringTrimLeft(s[1..])
+  else if IsJSWhitespace(s[0]) then StringTrimLeft(s[1..])
   else s
 }
 
 function StringTrimRight(s: string): string
   ensures |StringTrimRight(s)| <= |s|
+  ensures StringTrimRight(s) == "" || (|StringTrimRight(s)| > 0 && !IsJSWhitespace(StringTrimRight(s)[|StringTrimRight(s)|-1]))
   decreases |s|
 {
   if |s| == 0 then ""
-  else if s[|s|-1] == ' ' then StringTrimRight(s[..|s|-1])
+  else if IsJSWhitespace(s[|s|-1]) then StringTrimRight(s[..|s|-1])
   else s
 }
 
